src/temporal_logic/basic.lean
@@ -1,0 +1,477 @@
+
+import util.predicate
+
+@[user_attribute]
+meta def strengthening_attr : user_attribute :=
+{ name := `strengthening
+, descr := "
+Strenghtening lemmas to facilitate the stripping of small details in application.
+Expected shape `∀ p : pred' α, ⊩ f p ⟶ g p`
+" }
+
+namespace tactic.interactive
+open lean interactive.types
+open interactive lean.parser tactic
+open list (hiding map) has_map predicate
+local postfix *:9001 := many
+
+meta def apply_left (r : parse texpr) : tactic unit :=
+transitivity none ; [apply r >> done, skip]
+
+meta def apply_right (r : parse texpr) : tactic unit :=
+transitivity none ; [skip, apply r >> done]
+
+meta def references_to (v : expr) : tactic (list expr) :=
+do ctx ← local_context,
+   ctx_t ← mmap infer_type ctx,
+   return $ map prod.fst $ filter ((λ t, v.occurs t) ∘ prod.snd) $ zip ctx ctx_t
+
+-- meta def focus_rhs (tac : itactic) : tactic unit :=
+-- do `(_ ⟹ %%p) ← target <|> fail "expecting goal: _ ⟹ _",
+--    t ← infer_type p,
+--    q ← mk_meta_var t,
+--    e ← to_expr ``(%%q ⟹ %%p),
+--    h ← assert `h _, _
+
+meta def mk_local_hyp (a' : expr) (hyp : pexpr) : tactic (expr × expr × expr) :=
+do e' ← to_expr hyp,
+   e ← if e'.is_local_constant
+       then return e'
+       else note `h none e',
+   (expr.app f a)  ← infer_type e,
+   is_def_eq a a' <|> fail format!"{a} and {a'} are not the same argument",
+   return (e, f, a)
+
+meta def revert_pred (a : expr) (h : expr × expr × expr) : tactic unit :=
+do (expr.app g a') ← target,
+   is_def_eq a a',
+   tactic.revert h.1,
+   refine ``(impl_of_p_impl %%a _)
+   -- to_expr ``((%%h.2.1 ⟶ %%g) %%a) >>= tactic.change
+
+meta def revert_p (hyps : parse pexpr_list_or_texpr) : tactic unit :=
+do (expr.app g a) ← target,
+   hyps' ← mmap (mk_local_hyp a) hyps,
+   ls ← references_to a,
+   let vars := hyps'.map prod.fst,
+   mmap tactic.clear (ls.diff vars),
+   if a.is_local_constant then do -- <|> fail format!"{a} is not a local constant",
+     mmap' (revert_pred a) hyps',
+     () <$ tactic.revert a
+   else (mmap' (revert_pred a) hyps' >> tactic.generalize a),
+   -- to_expr ``(entails_of_forall_impl _) >>= infer_type >>= trace,
+   -- trace_state
+   tactic.refine ``(entails_of_forall_impl _)
+   -- to_expr ``(%%f ⟹ %%g) >>= tactic.change
+
+private meta def apply_trans : expr → expr → list expr → tactic unit
+ | _ _ [] := return ()
+ | p q (e :: es) := refine ``(@function.comp %%p %%e %%q _ _) ; [ skip , apply_trans p e es ]
+
+meta def imp_transitivity : parse (optional pexpr_list_or_texpr) → tactic unit
+ | none :=
+do `(%%p → %%q) ← target <|> fail "expecting implication",
+   refine ``(@function.comp %%p _ %%q _ _) >> rotate_left 1
+ | (some xs) :=
+do xs' ← mmap to_expr xs,
+   `(%%p → %%q) ← target <|> fail "expecting implication",
+   focus1 (apply_trans p q xs'.reverse)
+
+meta def apply' (e : parse texpr) : tactic unit :=
+apply e <|> (intro1 >>= λ h, (apply' ; try (tactic.exact h)) >> try (tactic.clear h))
+
+meta def TL_unfold (cs : parse ident*) (loc : parse location) : tactic unit :=
+do unfold_coes loc, unfold (cs ++ [`pred'.apply]) loc
+
+meta def coes_thms : list name :=
+[`predicate.lifted₀
+,`coe,`lift_t,`lift,`has_lift_t,`coe_t,`coe,`has_coe_t
+,`coe_b,`coe,`has_coe,`coe_fn,`coe,`has_coe_to_fun
+,`coe_sort,`coe,`has_coe_to_sort,`predicate.lifted₀]
+
+meta def TL_simp
+   (only_kw : parse only_flag)
+   (args : parse simp_arg_list)
+   (w : parse with_ident_list)
+   (loc : parse location) : tactic unit :=
+do std_lmm ← mmap (map (simp_arg_type.expr ∘ to_pexpr) ∘ mk_const) (coes_thms ++ [`predicate.pred'.apply,`temporal.init_to_fun]) ,
+   repeat (simp only_kw args w loc <|> simp only_kw std_lmm w loc <|> unfold_coes loc <|> unfold [`predicate.pred'.apply,`predicate.lifted₀] loc)
+
+end tactic.interactive
+
+
+-- section
+-- variables b : Prop
+-- variables c : ℕ → Prop
+-- variable h : b → ∀ i, c i
+-- variable h' : ℕ
+-- include h h'
+-- example : ∀ i, c i :=
+-- begin
+--   apply h , done,
+-- end
+
+-- end
+
+namespace temporal
+
+open predicate
+
+universe variables u u₀ u₁ u₂
+
+variables {α : Sort u₀} {β : Type u₁} {γ : Sort u₂}
+
+@[reducible]
+def cpred (β : Type u) := pred' (stream β)
+
+def act (β : Sort u) := β → β → Prop
+
+def action (a : act β) : cpred β :=
+⟨ λ τ, a (τ 0) (τ 1) ⟩
+
+def eventually (p : cpred β) : cpred β :=
+⟨ λ τ, ∃ i, p.apply (τ.drop i) ⟩
+def henceforth (p : cpred β) : cpred β :=
+⟨ λ τ, Π i, p.apply (τ.drop i) ⟩
+def next (p : cpred β) : cpred β :=
+⟨ λ τ, p.apply τ.tail ⟩
+def init (p : pred' β) : cpred β :=
+⟨ λ τ, p.apply (τ 0) ⟩
+
+prefix `•`:85 := init
+prefix `⊙`:90 := next
+prefix `◇`:95 := eventually -- \di
+prefix `◻`:95 := henceforth -- \sqw
+notation `⟦`:max act `⟧`:0 := action act
+-- notation `⦃` act `⦄`:95 := ew act
+
+lemma init_to_fun (p : pred' β) (τ : stream β) : (•p).apply τ = p.apply (τ 0) := rfl
+
+def tl_leads_to (p q : cpred β) : cpred β :=
+◻(p ⟶ ◇q)
+
+infix ` ~> `:55 := tl_leads_to
+
+@[reducible]
+def tl_imp (h p q : cpred β) : Prop :=
+ctx_impl (◻ h) p q
+
+lemma tl_imp_intro (h : cpred β) {p q : cpred β}
+  (h' : ◻h ⟹ (p ⟶ q))
+: tl_imp h p q :=
+begin
+  constructor, intro,
+  exact (h' True).apply σ trivial,
+end
+
+lemma tl_imp_elim (h : cpred β) {p q : cpred β}
+  (h' : tl_imp h p q)
+: ◻h ⟹ (p ⟶ q) :=
+begin
+  intro, revert Γ,
+  apply intro_p_imp h',
+end
+
+lemma tl_imp_intro' (h : cpred β) {p q : cpred β}
+  (h' : p ⟹ q)
+: tl_imp h p q :=
+h' _
+
+@[simp]
+lemma hence_true : ◻(True : cpred β) = True :=
+begin
+  funext1,
+  split ; intro h,
+  { trivial },
+  { intro, trivial }
+end
+
+lemma tl_imp_elim' {p q : cpred β}
+  (h : tl_imp True p q)
+: p ⟹ q :=
+begin
+  simp [tl_imp,ctx_impl] at h,
+  apply h,
+end
+
+@[strengthening]
+lemma eventually_weaken (p : cpred β)
+: (p ⟹ ◇ p) :=
+begin
+  pointwise with τ h,
+  unfold eventually pred'.apply,
+  existsi 0,
+  apply h
+end
+open stream
+-- lemma eventually_weaken' {p : cpred β} {τ} (i) :
+--   p (drop i τ) → (◇ p) τ :=
+-- begin
+--   intros h,
+--   TL_unfold eventually,
+--   existsi i,
+--   apply h
+-- end
+
+-- lemma eventually_of_next {p : cpred β}
+-- : ⊙p ⟹ ◇p :=
+-- sorry
+
+@[strengthening]
+lemma next_entails_eventually (p : cpred β)
+: ⊙p ⟹ ◇p :=
+sorry
+
+@[strengthening]
+lemma henceforth_str (p : cpred β) :
+  (◻p ⟹ p) :=
+begin
+  pointwise with τ h, apply h 0
+end
+
+-- lemma henceforth_str' {p : cpred β} {τ} (i) :
+--   (◻p) τ → p (drop i τ) :=
+-- begin
+--   intros h, apply h i
+-- end
+
+-- lemma henceforth_delay {p : cpred β} {τ} (i) :
+--   (◻p) τ → (◻p) (drop i τ) :=
+-- begin
+--   intros h j, simp [drop_drop], apply h
+-- end
+
+lemma init_eq_action {p : pred' β}
+: •(p : pred' β) = ⟦ λ s s', s ⊨ p ⟧ :=
+rfl
+
+lemma next_init_eq_action {p : pred' β}
+: ⊙•(p : pred' β) = ⟦ λ s s', s' ⊨ p ⟧ :=
+rfl
+
+lemma action_eq_next {p : β → β → Prop}
+:  (⟦ p ⟧ : cpred β) = (∃∃ s : β, •eq s ⋀ ⊙•p s) :=
+begin
+  funext τ, TL_unfold action p_exists pred.p_exists,
+  split
+  ; try {TL_simp [next]}
+  ; intros
+  ; try {subst x}
+  ; assumption,
+end
+
+lemma henceforth_next_intro (p : cpred β)
+: ◻p = ◻(p ⋀ ⊙p) := sorry
+
+@[simp]
+lemma eventually_eventually (p : cpred β) : ◇◇ p = ◇ p :=
+begin
+  funext τ,
+  split
+  ; unfold eventually
+  ; intro h
+  ; cases h with i h,
+  { cases h with j h,
+    existsi (j+i),
+    rw drop_drop at h,
+    apply h },
+  { existsi (0 : ℕ),
+    existsi i,
+    apply h }
+end
+
+@[simp]
+lemma henceforth_henceforth (p : cpred β) : ◻◻ p = ◻ p :=
+begin
+  funext _,
+  split
+  ; intro h,
+  { intro i,
+    have h' := h i 0,
+    simp [drop_drop] at h',
+    apply h' },
+  { intros i j,
+    simp [drop_drop],
+    apply h }
+end
+
+-- lemma henceforth_drop {p : cpred β} {τ} (i : ℕ) :
+-- (◻p) τ → (◻p) (τ.drop i) :=
+-- begin
+--   intro h,
+--   rw ← henceforth_henceforth at h,
+--   apply h,
+-- end
+
+/- True / False -/
+
+@[simp]
+lemma hence_false : ◻(False : cpred β) = False :=
+begin
+  funext _,
+  split ; intro h,
+  { cases h 0 },
+  { cases h }
+end
+
+@[simp]
+lemma event_false : ◇(False : cpred β) = False :=
+begin
+  funext _,
+  split ; intro h,
+  { cases h with _ h, cases h },
+  { cases h }
+end
+
+@[simp]
+lemma init_false : (•False) = (False : cpred β) :=
+begin
+  funext1,
+  split ; intro h,
+  { cases h },
+  { cases h }
+end
+
+@[simp]
+lemma eventually_true : ◇(True : cpred β) = True :=
+begin
+  funext1,
+  split ; intro h,
+  { trivial },
+  { apply exists.intro 0, trivial }
+end
+
+@[simp]
+lemma init_true : (•True) = (True : cpred β) :=
+begin
+  funext1,
+  split ; intro h ; trivial,
+end
+
+lemma init_exists {t} (p : t → pred' β)
+: •(∃∃ i, p i) = ∃∃ i, •p i :=
+begin
+  funext x,
+  TL_simp [p_exists,pred.p_exists,init]
+end
+
+/- monotonicity -/
+
+@[monotonic]
+lemma eventually_tl_imp_eventually {h p q : cpred β}
+  (f : tl_imp h p q)
+: tl_imp h (◇p) (◇q) :=
+begin
+  unfold tl_imp ctx_impl at ⊢ f,
+  pointwise f with τ h',
+  apply exists_imp_exists,
+  intro i,
+  apply f,
+  rw ← henceforth_henceforth at h',
+  apply h',
+end
+
+@[monotonic]
+lemma eventually_entails_eventually {p q : cpred β}
+  (f : p ⟹ q)
+: (◇p) ⟹ (◇q) :=
+begin
+  apply tl_imp_elim',
+  monotonicity (tl_imp_intro' _ f),
+end
+
+lemma eventually_imp_eventually {p q : cpred β} {Γ}
+ (f : Γ ⊢ ◻ (p ⟶ q))
+: Γ ⊢ (◇p) ⟶ (◇q) :=
+begin
+  constructor, introv hΓ,
+  apply exists_imp_exists,
+  intro i,
+  apply f.apply _ hΓ,
+end
+
+@[monotonic]
+lemma henceforth_tl_imp_henceforth {h p q : cpred β}
+  (f : tl_imp h p q)
+: tl_imp h (◻p) (◻q) :=
+begin
+  unfold tl_imp ctx_impl at *,
+  pointwise f with τ h',
+  TL_simp [henceforth], intro_mono i,
+  apply f ,
+  rw ← henceforth_henceforth at h',
+  apply  h',
+end
+
+@[monotonic]
+lemma henceforth_entails_henceforth {p q : cpred β}
+  (f : p ⟹ q)
+: (◻p) ⟹ (◻q) :=
+begin
+  refine tl_imp_elim' _,
+  monotonicity (tl_imp_intro' _ f),
+end
+
+lemma henceforth_imp_henceforth {p q : cpred β} {Γ}
+  (h : Γ ⊢ ◻ (p ⟶ q))
+: Γ ⊢ (◻p) ⟶ (◻q) :=
+begin
+  pointwise h with τ,
+  specialize h τ, simp [henceforth] at ⊢ h,
+  introv h₀ h₁,
+  auto,
+end
+
+@[monotonic]
+lemma init_entails_init {p q : pred' β} (f : p ⟹ q)
+: (•p) ⟹ (•q) :=
+begin
+  pointwise f with i,
+  xassumption,
+end
+
+lemma inf_often_entails_inf_often {p q : cpred β} (f : p ⟹ q)
+: ◻◇p ⟹ ◻◇q :=
+by monotonicity f
+
+lemma inf_often_entails_inf_often' {p q : pred' β} (f : p ⟹ q)
+: ◻◇•p ⟹ ◻◇•q :=
+by monotonicity f
+
+lemma stable_entails_stable {p q : cpred β} (f : p ⟹ q)
+: ◇◻p ⟹ ◇◻q :=
+by monotonicity f
+
+lemma stable_entails_stable' {p q : pred' β} (f : p ⟹ q)
+: ◇◻•p ⟹ ◇◻•q :=
+by monotonicity f
+
+lemma henceforth_and (p q : cpred β)
+: ◻(p ⋀ q) = ◻p ⋀ ◻q :=
+begin
+  funext1,
+  repeat { split ; intros }
+  ; intros i ; try { simp, split },
+  { apply (a i).left },
+  { apply (a i).right },
+  { apply a.left },
+  { apply a.right },
+end
+
+lemma henceforth_forall (P : α → cpred β)
+: ◻(∀∀ x, P x) = ∀∀ x, ◻P x :=
+begin
+  funext1,
+  TL_simp [henceforth,p_forall],
+  rw forall_swap,
+end
+
+@[simp]
+lemma not_eventually {β} (p : cpred β)
+: (-◇p) = (◻-p) :=
+begin
+  funext1,
+  TL_simp [henceforth,not_forall_iff_exists_not,eventually],
+end
+
+end temporal
